reorganize Rake (add sections, etc)

Rake.lean
@@ -1,9 +1,5 @@
 -- For the purposes of this library, a "Rake" is a sorted
 -- list of arithmetic sequences that share the same delta.
--- A rake can be combined with a Prop to form a RakeMap,
--- to model a bejection between the natural numbers and a
--- subset of the natural numbers with a lower bound and
--- the multiples certain numbers removed.
 import ASeq
 import MathLib.Data.List.Sort
 import Mathlib.Data.List.Dedup
@@ -23,104 +19,15 @@ def zer : Rake := { d := 0, ks := [0] }
 def nat : Rake := { d := 1, ks := [0] }
 def ge2 : Rake := { d := 1, ks := [2] }
 
-def sort_nodup (xs:List Nat) (hxs₀ : List.Nodup xs)
-: { xs':List Nat // List.Sorted (·<·) xs' ∧ xs'.length = xs.length } :=
-  let xs' := xs.mergeSort (·≤·)
-  have hnodup : xs'.Nodup := xs.perm_mergeSort (·≤·) |>.nodup_iff |>.mpr hxs₀
-  have hsorted: List.Sorted (·≤·) xs' := List.sorted_mergeSort (·≤·) xs
-  have hlength := by simp_all only [List.length_mergeSort, xs']
-  ⟨xs', And.intro (List.Sorted.lt_of_le hsorted hnodup) hlength⟩
+section « terms » -- generating output terms from the rake
 
 def term (r: Rake) (n : Nat) : Nat :=
   let q := r.ks.length
   have : n%q < r.ks.length := Nat.mod_lt _ r.hsize
   aseq r.ks[n%q] r.d |>.term (n/q)
 
-def sort (r: Rake) : {r':Rake // r'.sorted } :=
-  if h: r.sorted then ⟨r, h⟩
-  else
-    let ks₀ := r.ks
-    let ks₁ := ks₀.dedup
-    let ks₂ := sort_nodup ks₁ ks₀.nodup_dedup
-  have hlen₁ : ks₁.length ≠ 0 := by have:=r.hsize; aesop
-  have hsize := Nat.lt_of_lt_of_eq (Nat.zero_lt_of_ne_zero hlen₁) ks₂.prop.right.symm
-  ⟨{ d:=r.d, ks:=ks₂, hsort:=λ_=>ks₂.prop.left, hsize := hsize}, rfl⟩
-
-lemma length_pos_of_dedup {l:List Nat} (hlen: 0 < l.length) : 0 < l.dedup.length := by
-  obtain ⟨hd, tl, hcons⟩ := List.exists_cons_of_length_pos hlen
-  have : hd ∈ l := by rw[hcons]; exact List.mem_cons_self hd tl
-  rw[←List.mem_dedup] at this
-  exact List.length_pos_of_mem this
-
-def gte (r: Rake) (n: Nat) : Rake  :=
-  let f : ℕ → ℕ := (λk => let s := aseq k r.d; (ASeq.gte s n).k)
-  { d := r.d, ks := r.ks.map f, sorted := false,
-    hsize := Nat.lt_of_lt_of_eq r.hsize (r.ks.length_map _).symm }
-
-def seq (r:Rake) (n:Nat) {hn:n<r.ks.length} : ASeq :=
-  aseq (r.ks[n]'hn) r.d
-
-def seqs (r: Rake) : List ASeq :=
-  r.ks.map (λ k => aseq k r.d)
-
-/--
-Partition each sequence in the rake by partitioning their *inputs*
-into equivalance classes mod n. This multiplies the number of sequences
-by n. We can't allow n to be zero because then we'd have no sequences left,
-and this would break the guarantee that term (n) < term n+1. -/
-def partition (r: Rake) (n: Nat) (hn: 0 < n): Rake :=
-  let seqs' := r.seqs.map (λ s => s.partition n) |>.join
-  let ks₀ := seqs'.map (λ s => s.k)
-  -- aseq.partiton n  always produces a list of length n
-  have hsize := by
-    have hlen₀: 0 < seqs'.length := by
-      unfold_let; rw[List.length_join']; simp
-      have : (List.length ∘ λs:ASeq=> s.partition n) = λ_ => n := by
-        calc (List.length ∘ λ s => s.partition n)
-          _ = λs:ASeq => (s.partition n).length := by rfl
-          _ = λ_:ASeq => n := by conv=> lhs; simp[ASeq.length_partition]
-      have : 0 < r.seqs.length := by unfold seqs; simp[List.length_map, r.hsize]
-      simp_all -- this introduces "replicate" because the lengths are all the same.
-      show 0 < Nat.sum (List.replicate r.seqs.length n)
-      have sum_rep {x y: Nat} : Nat.sum (List.replicate x y) = x*y := by
-        induction x; simp_all; case succ hx => simp[hx]; linarith
-      simp_all
-    have : ks₀.length = seqs'.length := List.length_map seqs' _
-    aesop
-  { d := r.d * n, ks := ks₀, sorted := false, hsize := hsize }
-
-def rem (r : Rake) (n : Nat) : Rake :=
-  if hn₀ : n = 0 then r.gte 1
-  else
-    have hn : 0 < n := Nat.zero_lt_of_ne_zero hn₀
-    let gcd := r.d.gcd n
-    have hz : 0 < (n/gcd) := Nat.div_gcd_pos_of_pos_right r.d hn
-    let r' := if n∣r.d then r else r.partition (n/gcd) hz
-    let ks := r'.ks |>.filter (λk => ¬n∣k)
-    if hlen: ks.length = 0 then zer
-    else { d := r'.d, ks:=ks, sorted := false, hsize := Nat.zero_lt_of_ne_zero hlen }
-
-/-- proof that if a rake produces a term, it's because one of the sequences
-    it contains produces that term. -/
-lemma ___unused______ex_seq (r: Rake)
-  : (r.term m = n) → (∃k ∈ r.ks, n = k + r.d * (m/r.ks.length)) := by
-  unfold term; intro hmn; simp_all
-  let q := r.ks.length
-  have hmq: m%q < r.ks.length := Nat.mod_lt _ r.hsize
-  let k := r.ks[m%q]; use k
-  apply And.intro
-  · show k ∈ r.ks
-    exact List.get_mem r.ks (m % q) hmq
-  · show n = k + r.d * (m/q)
-    calc
-      n = (aseq r.ks[m%q] r.d).term (m/q) := by simp[hmn]
-      _ = (aseq k r.d).term (m/q) := by rfl
-      _ = k + r.d * (m/q) := by unfold aseq ASeq.term; simp_all
-
-theorem div_lt_of_lt_mod_eq {m n d:Nat} {hdpos: 0 < d} {hmn: m<n} : (m%d = n%d) → (m/d < n/d) := by
-  intro hmod
-  rw[←m.div_add_mod d, ←n.div_add_mod d, hmod, Nat.add_lt_add_iff_right] at hmn
-  exact (Nat.mul_lt_mul_left hdpos).mp hmn
+def terms (r: Rake) (n: Nat) : List Nat :=
+  List.range n |>.map r.term
 
 theorem term_simp (r:Rake) (n:Nat)
 : (∃k, (r.term n = k + r.d * (n/r.ks.length)) ∧ ∃i: Fin r.ks.length, i=n%r.ks.length ∧ k=r.ks[i]) := by
@@ -168,10 +75,61 @@ theorem term_iff (r:Rake)
     rw[Nat.add_mul_div_right i.val x r.hsize, ←hi₁, Nat.mul_comm]
     simp; exact hx
 
-lemma sorted_indices (xs:List Nat) {hsort: List.Sorted (·<·) xs} (i j:Nat) (hij: i<j) (hj: j<xs.length)
-  : (xs[i]'(by omega) < xs[j]'hj) := by
-  conv at hsort => dsimp[List.Sorted]; rw[List.pairwise_iff_get]
-  simp_all
+end « terms »
+
+section « sequences » -- arithmetic sequences for each k ∈ ks
+
+def seq (r:Rake) (n:Nat) {hn:n<r.ks.length} : ASeq :=
+  aseq (r.ks[n]'hn) r.d
+
+def seqs (r: Rake) : List ASeq :=
+  r.ks.map (λ k => aseq k r.d)
+
+/-- proof that if a rake produces a term, it's because one of the sequences
+    it contains produces that term. -/
+
+theorem unused__ex_seq (r: Rake)
+  : (r.term m = n) → (∃k ∈ r.ks, n = k + r.d * (m/r.ks.length)) := by
+  unfold term; intro hmn; simp_all
+  let q := r.ks.length
+  have hmq: m%q < r.ks.length := Nat.mod_lt _ r.hsize
+  let k := r.ks[m%q]; use k
+  apply And.intro
+  · show k ∈ r.ks
+    exact List.get_mem r.ks (m % q) hmq
+  · show n = k + r.d * (m/q)
+    calc
+      n = (aseq r.ks[m%q] r.d).term (m/q) := by simp[hmn]
+      _ = (aseq k r.d).term (m/q) := by rfl
+      _ = k + r.d * (m/q) := by unfold aseq ASeq.term; simp_all
+
+end « sequences »
+
+section « sort and dedup »
+
+def sort_nodup (xs:List Nat) (hxs₀ : List.Nodup xs)
+: { xs':List Nat // List.Sorted (·<·) xs' ∧ xs'.length = xs.length } :=
+  let xs' := xs.mergeSort (·≤·)
+  have hnodup : xs'.Nodup := xs.perm_mergeSort (·≤·) |>.nodup_iff |>.mpr hxs₀
+  have hsorted: List.Sorted (·≤·) xs' := List.sorted_mergeSort (·≤·) xs
+  have hlength := by simp_all only [List.length_mergeSort, xs']
+  ⟨xs', And.intro (List.Sorted.lt_of_le hsorted hnodup) hlength⟩
+
+def sort (r: Rake) : {r':Rake // r'.sorted } :=
+  if h: r.sorted then ⟨r, h⟩
+  else
+    let ks₀ := r.ks
+    let ks₁ := ks₀.dedup
+    let ks₂ := sort_nodup ks₁ ks₀.nodup_dedup
+  have hlen₁ : ks₁.length ≠ 0 := by have:=r.hsize; aesop
+  have hsize := Nat.lt_of_lt_of_eq (Nat.zero_lt_of_ne_zero hlen₁) ks₂.prop.right.symm
+  ⟨{ d:=r.d, ks:=ks₂, hsort:=λ_=>ks₂.prop.left, hsize := hsize}, rfl⟩
+
+lemma length_pos_of_dedup {l:List Nat} (hlen: 0 < l.length) : 0 < l.dedup.length := by
+  obtain ⟨hd, tl, hcons⟩ := List.exists_cons_of_length_pos hlen
+  have : hd ∈ l := by rw[hcons]; exact List.mem_cons_self hd tl
+  rw[←List.mem_dedup] at this
+  exact List.length_pos_of_mem this
 
 def zero_le_cases (n:Nat) (zeq: 0=n → P) (zlt: 0<n → P) : P :=
   if h:0=n then zeq h else zlt <| Nat.zero_lt_of_ne_zero λa=>h a.symm
@@ -198,3 +156,63 @@ theorem sorted_min_term_zero (r: Rake) (hr: r.sorted) : ∀ n, (r.term 0 ≤ r.t
   case zlt =>
     have : i₀.val < i₁.val := by aesop
     exact Nat.le_of_succ_le <| sorted_get r.ks (r.hsort hr) i₀ i₁ this
+
+end « sort and dedup »
+
+section « rake operations »
+
+section « partition »
+/--
+Partition each sequence in the rake by partitioning their *inputs*
+into equivalance classes mod n. This multiplies the number of sequences
+by n. We can't allow n to be zero because then we'd have no sequences left,
+and this would break the guarantee that term (n) < term n+1. -/
+def partition (r: Rake) (n: Nat) (hn: 0 < n): Rake :=
+  let seqs' := r.seqs.map (λ s => s.partition n) |>.join
+  let ks₀ := seqs'.map (λ s => s.k)
+  -- aseq.partiton n  always produces a list of length n
+  have hsize := by
+    have hlen₀: 0 < seqs'.length := by
+      unfold_let; rw[List.length_join']; simp
+      have : (List.length ∘ λs:ASeq=> s.partition n) = λ_ => n := by
+        calc (List.length ∘ λ s => s.partition n)
+          _ = λs:ASeq => (s.partition n).length := by rfl
+          _ = λ_:ASeq => n := by conv=> lhs; simp[ASeq.length_partition]
+      have : 0 < r.seqs.length := by unfold seqs; simp[List.length_map, r.hsize]
+      simp_all -- this introduces "replicate" because the lengths are all the same.
+      show 0 < Nat.sum (List.replicate r.seqs.length n)
+      have sum_rep {x y: Nat} : Nat.sum (List.replicate x y) = x*y := by
+        induction x; simp_all; case succ hx => simp[hx]; linarith
+      simp_all
+    have : ks₀.length = seqs'.length := List.length_map seqs' _
+    aesop
+  { d := r.d * n, ks := ks₀, sorted := false, hsize := hsize }
+
+end « partition »
+
+section « rem (remove multiples) »
+
+/-- remove all multiples of `n`. if `n=0`, `Rake.zer` is returned. -/
+def rem (r : Rake) (n : Nat) : Rake :=
+  if hn₀ : n = 0 then zer
+  else
+    have hn : 0 < n := Nat.zero_lt_of_ne_zero hn₀
+    let gcd := r.d.gcd n
+    have hz : 0 < (n/gcd) := Nat.div_gcd_pos_of_pos_right r.d hn
+    let r' := if n∣r.d then r else r.partition (n/gcd) hz
+    let ks := r'.ks |>.filter (λk => ¬n∣k)
+    if hlen: ks.length = 0 then zer
+    else { d := r'.d, ks:=ks, sorted := false, hsize := Nat.zero_lt_of_ne_zero hlen }
+
+end « rem (remove multiples) »
+
+section « gte (greater than or equal to) »
+
+def gte (r: Rake) (n: Nat) : Rake  :=
+  let f : ℕ → ℕ := (λk => let s := aseq k r.d; (ASeq.gte s n).k)
+  { d := r.d, ks := r.ks.map f, sorted := false,
+    hsize := Nat.lt_of_lt_of_eq r.hsize (r.ks.length_map _).symm }
+
+end « gte (greater than or equal to) »
+
+end « rake operations »
